monadproofs/proofs/execproofs/exec_transactions.v
@@ -1,0 +1,35 @@
+Require Import monad.proofs.misc.
+Require Import monad.proofs.libspecs.
+Require Import monad.proofs.evmopsem.
+Import linearity.
+Require Import bedrock.auto.invariants.
+Require Import bedrock.auto.cpp.proof.
+
+Require Import bedrock.auto.cpp.tactics4.
+Require Import monad.asts.exb.
+Require Import monad.proofs.exec_specs.
+
+
+Section with_Sigma.
+  Context `{Sigma:cpp_logic} {CU: genv} {hh: HasOwn mpredI fracR}.
+  Context  {MODd : exb.module ⊧ CU}.
+
+
+  Existing Instance learnArrUnsafe.
+  Existing Instance learnpArrUnsafe.
+
+Lemma prf: denoteModule module
+             ** tvector_spec
+             ** reset_promises
+             ** fork_task
+             ** vector_op_monad
+             ** recover_sender
+             ** opt_move_assign
+             ** wait_for_promise
+             ** set_value
+             ** destrop
+             |-- exect.
+Proof using MODd.
+Abort.
+End with_Sigma.
+
